# Exercise

Prove that $\sum^{n}_{i=1}i^3=n^2(n+1)^2/4$ for $n \ge 0$, by induction.

# Solution

## Base case:

On the left-hand side:

For n = 0:

$\sum\limits_{i=1}^0 i^3 = 0$

On the right-hand side:

For n = 0:

$\frac{0^2(0+1)^2}{4} = 0$

So for n = 0, the formula holds.

## Inductive hypothesis:

Assume that for $k \ge 0$, the formula becomes:

$\sum\limits_{i=1}^{k} i^3 = \frac{k^2(k+1)^2}{4}$.

## Inductive step:

We must prove the formula still holds for $k+1$.

For $k+1$ the formula need to be:

$\sum\limits_{i=1}^{k+1} i^3 = \frac{(k+1)^2(k+2)^2}{4}$.

On the left-hand side:

$\sum\limits_{i=1}^{k+1} i^3 = \sum\limits_{i=1}^{k} i^3 + (k+1)^3$

$= \frac{k^2(k+1)^2}{4} + (k+1)^3$.

$= (k+1)^2(\frac{k^2}{4} + (k+1))$.

$= (k+1)^2(\frac{k^2 + 4k + 4}{4})$.

On the right-hand side:

$\frac{(k+1)^2(k+2)^2}{4} = \frac{(k+1)^2(k^2 + 4k + 4)}{4}$


so for $k+1$ the formula still holds.




