# Exercise

Prove that $\sum^{n}_{i=1}i^2=n(n+1)(2n+1)/6$ for $n \ge 0$, by induction.

# Solution

## Base case:

On the left-hand side:

For n = 0:

$\sum\limits_{i=1}^0 i^2 = 0$

On the right-hand side:

For n = 0:

$\frac{0(0+1)(2*0+1)}{6} = 0$

So for n = 0, the formula holds.

## Inductive hypothesis:

Assume that for $k \ge 0$, the formula becomes:

$\sum\limits_{i=1}^{k} i^2 = \frac{k(k+1)(2k+1)}{6}$.

## Inductive step:

We must prove the formula still holds for $k+1$.

For $k+1$ the formula need to be:

$\sum\limits_{i=1}^{k+1} i^2 = \frac{(k+1)(k+2)(2k+3)}{6}$.

On the left-hand side:

$\sum\limits_{i=1}^{k+1} i^2 = \sum\limits_{i=1}^{k} i^2 + (k+1)^2$

$= (k+1) (\frac{2k^2 + 7k + 6}{6})$.


On the right-hand side:

$\frac{(k+1)(k+2)(2k+3)}{6} = \frac{(k+1)(2k^2+3k+4k+6)}{6}$.

so for $k+1$ the formula still holds.




