# Exercise

Prove that $\sum^{n}_{i=1} i = n(n+1)/2$ for $n \ge 0$, by induction.

# Solution

## Base case:

For n = 0 on the left side.

$\sum\limits_{i=1}^0 i = 0$

For n = 0 on the right side.

$
\frac{0(0+1)}{2} = 0
$

## Inductive hypothesis:

Assume that for some $k \ge 0$,

$\sum\limits_{i=1}^k i = \frac{k(k+1)}{2} .$

## Inductive step:

For $k + 1$, it becomes

$\sum\limits_{i=1}^{k+1} i = \frac{(k+1)(k+2)}{2}$.

First, from the left side:

$\sum\limits_{i=1}^{k+1} = (\sum\limits_{i=1}^{k} i) + (k+1)$.

By the hypothesis:

$=\frac{k(k+1)}{2} + (k+1) = \frac{k(k+1)+2(k+1)}{2} = \frac{(k+1)(k+2)}{2}$.

So the formula holds for $k+1$.

## Conclusion

$\sum\limits_{i=1}^n i = \frac{n(n+1)}{2} for all n \ge 0$.__